pallene.v
@@ -11,24 +11,24 @@ Require Import LIR.maps.
 Require Import LIR.lir.
 
 
-Inductive TPall : Set :=
-| TPstar : TPall | TPnil : TPall | TPint : TPall
-| TParr : TPall -> TPall | TPfun : TPall -> TPall -> TPall
+Inductive PType : Set :=
+| PTStar : PType | PTNil : PType | PTInt : PType
+| TParr : PType -> PType | TPfun : PType -> PType -> PType
 .
 
 
-Fixpoint TPeq (t1 t2 : TPall) : bool :=
+Fixpoint TPeq (t1 t2 : PType) : bool :=
   match t1, t2 with
-  | TPstar, TPstar => true
-  | TPnil, TPnil => true
-  | TPint, TPint => true
+  | PTStar, PTStar => true
+  | PTNil, PTNil => true
+  | PTInt, PTInt => true
   | TParr t1', TParr t2' => TPeq t1' t2'
   | TPfun t1' t1'', TPfun t2' t2'' => TPeq t1' t2' && TPeq t1'' t2''
   | _, _ => false
   end.
 
 
-Lemma dec_TP : forall (t1 t2 : TPall), TPeq t1 t2 = true <-> t1 = t2.
+Lemma dec_TP : forall (t1 t2 : PType), TPeq t1 t2 = true <-> t1 = t2.
 Proof.
   split.
   - generalize dependent t2.
@@ -45,94 +45,94 @@ Lemma TPeqRefl : forall t, TPeq t t = true.
 Proof. intros t. apply dec_TP. trivial. Qed.
 
 
-Definition Environment := Map TPall.
+Definition Environment := Map PType.
 
-Inductive EPall : Set :=
-| EPnil : EPall
-| EPnum : nat -> EPall
-| EPplus : EPall -> EPall -> EPall
-| EPnew : TPall -> EPall
-| EPget : EPall -> EPall -> EPall
-| EPset : EPall -> EPall -> EPall -> EPall
-| EPvar : string -> EPall
-| EPapp :  EPall -> EPall -> EPall
-| EPfunc : string -> TPall -> EPall -> EPall
-| EPcast : EPall -> TPall -> EPall
+Inductive PE : Set :=
+| PENil : PE
+| PENum : nat -> PE
+| PEPlus : PE -> PE -> PE
+| PENew : PType -> PE
+| PEGet : PE -> PE -> PE
+| PESet : PE -> PE -> PE -> PE
+| PEVar : string -> PE
+| PEApp :  PE -> PE -> PE
+| PEFun : string -> PType -> PE -> PE
+| PECast : PE -> PType -> PE
 .
 
 
 Reserved Notation "Γ '|=' e ':' t"  (at level 40, no associativity,
                                      e at next level).
 
-Inductive PTyping : Environment -> EPall -> TPall -> Prop :=
-| PTyPnil : forall Γ, Γ |= EPnil : TPnil
-| PTyInt : forall Γ n, Γ |= EPnum n : TPint
+Inductive PTyping : Environment -> PE -> PType -> Prop :=
+| PTyNil : forall Γ, Γ |= PENil : PTNil
+| PTyInt : forall Γ n, Γ |= PENum n : PTInt
 | PTyVal : forall Γ var T,
     In Γ var = Some T ->
-    Γ |= EPvar var : T
-| PTyAdd : forall Γ e1 e2,
-    Γ |= e1 : TPint ->
-    Γ |= e2 : TPint ->
-    Γ |= EPplus e1 e2 : TPint
-| PTyNew : forall Γ T, Γ |= EPnew T : TParr T
+    Γ |= PEVar var : T
+| PTyPlus : forall Γ e1 e2,
+    Γ |= e1 : PTInt ->
+    Γ |= e2 : PTInt ->
+    Γ |= PEPlus e1 e2 : PTInt
+| PTyNew : forall Γ T, Γ |= PENew T : TParr T
 | PTyGet : forall Γ e1 T e2,
     Γ |= e1 : TParr T ->
-    Γ |= e2 : TPint ->
-    Γ |= EPget e1 e2 : T
+    Γ |= e2 : PTInt ->
+    Γ |= PEGet e1 e2 : T
 | PTySet : forall Γ e1 T e2 e3,
     Γ |= e1 : TParr T ->
-    Γ |= e2 : TPint ->
+    Γ |= e2 : PTInt ->
     Γ |= e3 : T ->
-    Γ |= EPset e1 e2 e3 : TPnil
+    Γ |= PESet e1 e2 e3 : PTNil
 | PTyFun : forall Γ var Tvar body Tbody,
     var |=> Tvar; Γ |= body : Tbody ->
-    Γ |= EPfunc var Tvar body : TPfun Tvar Tbody
+    Γ |= PEFun var Tvar body : TPfun Tvar Tbody
 | PTyApp : forall Γ e1 e2 T1 T2,
     Γ |= e1 : TPfun T1 T2 ->
     Γ |= e2 : T1 ->
-    Γ |= EPapp e1 e2 : T2
+    Γ |= PEApp e1 e2 : T2
 | PTyCast : forall Γ e T1 T2,
     Γ |= e : T1 ->
-    Γ |= EPcast e T2 : T2
+    Γ |= PECast e T2 : T2
 
 where "Γ '|=' e ':' t" := (PTyping Γ e t)
 .
 
 
-Fixpoint typeOf Γ e : option TPall :=
+Fixpoint typeOf Γ e : option PType :=
   match e with
-  | EPnil => Some TPnil
-  | EPnum _ => Some TPint
-  | EPplus e1 e2 =>
+  | PENil => Some PTNil
+  | PENum _ => Some PTInt
+  | PEPlus e1 e2 =>
     match (typeOf Γ e1), (typeOf Γ e2) with
-    | Some TPint, Some TPint => Some TPint
+    | Some PTInt, Some PTInt => Some PTInt
     | _, _ => None
     end
-  | EPnew T => Some (TParr T)
-  | EPget e1 e2 =>
+  | PENew T => Some (TParr T)
+  | PEGet e1 e2 =>
     match (typeOf Γ e1), (typeOf Γ e2) with
-    | Some (TParr T), Some TPint => Some T
+    | Some (TParr T), Some PTInt => Some T
     | _, _ => None
     end
-  | EPset e1 e2 e3 =>
+  | PESet e1 e2 e3 =>
     match (typeOf Γ e1), (typeOf Γ e2), (typeOf Γ e3) with
-    | Some (TParr T), Some TPint, Some T' =>
-        if TPeq T T' then Some TPnil else None
+    | Some (TParr T), Some PTInt, Some T' =>
+        if TPeq T T' then Some PTNil else None
     | _, _, _ => None
     end
-  | EPvar var => In Γ var
-  | EPapp e1 e2 =>
+  | PEVar var => In Γ var
+  | PEApp e1 e2 =>
     match typeOf Γ e1, typeOf Γ e2 with
     | Some (TPfun T1 T2), Some T1' =>
         if TPeq T1 T1' then Some T2 else None
     | _, _ => None
     end
-  | EPfunc var Tv e =>
+  | PEFun var Tv e =>
     match typeOf (var |=> Tv; Γ) e with
     | Some Tb => Some (TPfun Tv Tb)
     | None => None
     end
-  | EPcast e T =>
+  | PECast e T =>
     match typeOf Γ e with
     | Some _ => Some T
     | None => None
@@ -167,18 +167,15 @@ Proof.
   - destTOf Γ e1.
     destTOf Γ e2.
     destruct (typeOf Γ e3) eqn:?; try easy.
-    destruct (TPeq t t0) eqn:?; try easy.
-    inversion Heq; subst.
-    assert(t = t0). { apply dec_TP. trivial. }
-    subst. eauto using PTyping.
+    destruct (TPeq p p0) eqn:?; try easy.
+    assert(p = p0) by (apply dec_TP; trivial).
+    inversion Heq; subst. eauto using PTyping.
   - destTOf Γ e1.
     destruct (typeOf Γ e2) eqn:?; try easy.
-    destruct (TPeq t t1) eqn:?; try easy.
-    inversion Heq; subst. econstructor.
-    eapply IHe1. eauto.
-    assert (t = t1). { apply dec_TP. trivial. }
-    subst. auto.
-  - destruct (typeOf (s |=> t; Γ) e) eqn:?; try easy.
+    destruct (TPeq p p1) eqn:?; try easy.
+    assert (p = p1) by (apply dec_TP; trivial).
+    inversion Heq; subst. eauto using PTyping.
+  - destruct (typeOf (s |=> p; Γ) e) eqn:?; try easy.
     inversion Heq; subst. eauto using PTyping.
   - destruct (typeOf Γ e) eqn:?; try easy.
     inversion Heq; subst. eauto using PTyping.
@@ -189,17 +186,17 @@ Proof. split; auto using typeOfCorrect', typeOfCorrect''. Qed.
 
 
 
-Fixpoint TP2FCT (t : TPall) : FCType :=
+Fixpoint TP2FCT (t : PType) : IRType :=
   match t with
-  | TPstar => Tstar
-  | TPnil => Tgnil
-  | TPint => Tgint
-  | TParr _ => Tgtbl
-  | TPfun _ _ =>  Tgfun
+  | PTStar => IRTStar
+  | PTNil => TgNil
+  | PTInt => TgInt
+  | TParr _ => TgTbl
+  | TPfun _ _ =>  TgFun
   end.
 
 
-Fixpoint TP2TGamma (Γ : Map TPall) : Map FCType :=
+Fixpoint TP2TGamma (Γ : Map PType) : Map IRType :=
   match Γ with
   | MEmpty => MEmpty
   | MCons var T Γ' => MCons var (TP2FCT T) (TP2TGamma Γ')
@@ -209,20 +206,19 @@ Fixpoint TP2TGamma (Γ : Map TPall) : Map FCType :=
 Lemma TP2TGammaIn : forall Γ var T,
     In Γ var = Some T -> In (TP2TGamma Γ) var = Some (TP2FCT T).
 Proof.
-  induction Γ; intros var T H.
-  - simpl in *. easy.
-  - simpl in *. destruct (string_dec var s); subst; auto.
-    congruence.
+  induction Γ; intros var T H; simpl in *.
+  - easy.
+  - destruct (string_dec var s); auto; congruence.
 Qed.
 
 
-Definition Cast (t1 t2 : FCType) (e : LirExp) : LirExp :=
+Definition Cast (t1 t2 : IRType) (e : IRE) : IRE :=
   match t1, t2 with
-  | Tstar, Tstar => e
-  | Tstar, Ttag t => Ebox t e
-  | Ttag t, Tstar => Eunbox t e
-  | Ttag t1', Ttag t2' => if dec_Tag t1' t2' then e
-                            else Eunbox t1' (Ebox t2' e)
+  | IRTStar, IRTStar => e
+  | IRTStar, IRTTag t => IREBox t e
+  | IRTTag t, IRTStar => IREUnbox t e
+  | IRTTag t1', IRTTag t2' => if dec_Tag t1' t2' then e
+                            else IREUnbox t1' (IREBox t2' e)
   end.
 
 
@@ -231,88 +227,87 @@ Notation "'<' t1 '<=' t2 '>' e" := (Cast t1 t2 e)
 
 
 
-Definition tagOf Γ e : FCType :=
+Definition tagOf Γ e : IRType :=
   match typeOf Γ e with
   | Some T => TP2FCT T
-  | None => Tgnil
+  | None => TgNil
   end.
 
 Lemma tagOfT : forall Γ e T, typeOf Γ e = Some T -> tagOf Γ e = TP2FCT T.
 Proof. intros. unfold tagOf. rewrite H. trivial. Qed.
 
 
-Fixpoint Pall2Lir (Γ : Environment) (e : EPall) : LirExp :=
+Fixpoint Pall2Lir (Γ : Environment) (e : PE) : IRE :=
   match e with
-  | EPnil => Enil
-  | EPnum a => Enum a
-  | EPplus e1 e2 => Eplus (Pall2Lir Γ e1) (Pall2Lir Γ e2)
-  | EPnew _ => Ecstr
-  | EPget e1 e2 =>
-         <tagOf Γ e <= Tstar> (Eindx (Pall2Lir Γ e1) (Pall2Lir Γ e2))
-  | EPset e1 e2 e3 =>
-         (Eassg (Pall2Lir Γ e1)
-               (Pall2Lir Γ e2)
-                (<Tstar <= tagOf Γ e3> Pall2Lir Γ e3))
-  | EPvar var => Evar var
-  | EPfunc var T e => let Γ' := (var |=> T; Γ) in
-        Efun (Elambda var Tstar
-                      (Elambapp (Elambda var (TP2FCT T)
-                                    (<Tstar <= tagOf Γ' e> (Pall2Lir Γ' e)))
-                                (<TP2FCT T <= Tstar> (Evar var))))
-  | EPapp e1 e2 => <tagOf Γ e <= Tstar>
-         (Efunapp (Pall2Lir Γ e1)
-                  (<Tstar <= (tagOf Γ e2)> Pall2Lir Γ e2))
-  | EPcast e1 t => <TP2FCT t <= tagOf Γ e1> (Pall2Lir Γ e1)
+  | PENil => IRENil
+  | PENum a => IRENum a
+  | PEPlus e1 e2 => IREPlus (Pall2Lir Γ e1) (Pall2Lir Γ e2)
+  | PENew _ => IRECnst
+  | PEGet e1 e2 =>
+         <tagOf Γ e <= IRTStar> (IREGet (Pall2Lir Γ e1) (Pall2Lir Γ e2))
+  | PESet e1 e2 e3 =>
+         (IRESet (Pall2Lir Γ e1)
+                 (Pall2Lir Γ e2)
+                 (<IRTStar <= tagOf Γ e3> Pall2Lir Γ e3))
+  | PEVar var => IREVar var
+  | PEFun var T e => let Γ' := (var |=> T; Γ) in
+        IREFun (IRELamb var IRTStar
+                      (IRELambApp (IRELamb var (TP2FCT T)
+                                  (<IRTStar <= tagOf Γ' e> (Pall2Lir Γ' e)))
+                                  (<TP2FCT T <= IRTStar> (IREVar var))))
+  | PEApp e1 e2 => <tagOf Γ e <= IRTStar>
+         (IREFunApp (Pall2Lir Γ e1)
+                  (<IRTStar <= (tagOf Γ e2)> Pall2Lir Γ e2))
+  | PECast e1 t => <TP2FCT t <= tagOf Γ e1> (Pall2Lir Γ e1)
   end.
 
 
-Theorem Pall2LirWellTyped : forall Γ (e : EPall) T,
-    Γ |= e : T -> Typing (TP2TGamma Γ) (Pall2Lir Γ e) (TP2FCT T).
+Lemma invertCall : forall Γ e1 e2 T1 T2 t,
+  typeOf Γ e1 = Some (TPfun T1 T2) -> typeOf Γ e2 = Some T1 ->
+    tagOf Γ (PEApp e1 e2) = t -> TP2FCT T2 = t.
 Proof.
+  intros Γ e1 r2 T1 T2 t H1 H2.
+  unfold tagOf. simpl. rewrite H1. rewrite H2.
+  rewrite TPeqRefl. congruence.
+Qed.
+
+
+Ltac breakTagOf :=
+  match goal with
+  [H: typeOf _ ?E = Some ?T |- context C [tagOf _ ?E] ] =>
+    apply tagOfT in H; rewrite H; destruct (TP2FCT T) eqn:?;
+    eauto using IRTyping
+  end.
+
+
+Theorem Pall2LirWellTyped : forall Γ (e : PE) T,
+    Γ |= e : T -> IRTyping (TP2TGamma Γ) (Pall2Lir Γ e) (TP2FCT T).
+Proof with eauto using IRTyping.
   intros Γ e T H.
   induction H; simpl in *;
+  eauto using IRTyping,TP2TGammaIn;
   repeat match goal with
   | [H: PTyping ?G ?E ?T |- _] =>
       apply typeOfCorrect in H
-  end;
-  eauto using Typing,TP2TGammaIn.
+  end.
   - unfold tagOf. simpl. rewrite H. rewrite H0.
-    destruct (TP2FCT T) eqn:HTT; simpl; eauto using Typing.
+    destruct (TP2FCT T) eqn:?; simpl...
   - unfold tagOf. rewrite H1.
-    destruct (TP2FCT T) eqn:?; simpl; eauto using Typing.
-  - apply TyFun. apply TyLam. apply TyLamApp with (TP2FCT Tvar).
-    apply TyLam.
+    destruct (TP2FCT T) eqn:?; simpl...
+  - apply IRTyFun. apply IRTyLamb. apply IRTyLambApp with (TP2FCT Tvar).
+    apply IRTyLamb.
     + apply envExt with (var |=> TP2FCT Tvar; TP2TGamma Γ).
       apply inclusion_shadow'.
-      apply tagOfT in H. rewrite H.
-      destruct (TP2FCT Tbody) eqn:?; eauto using Typing.
+      breakTagOf.
     + apply tagOfT in H;
       destruct (TP2FCT Tvar) eqn:?;
-      eauto using Typing,InEq.
-  - destruct (tagOf Γ (EPapp e1 e2)) eqn:?.
-    + assert (Ttag t = TP2FCT T2).
-      { unfold tagOf in Heqf. simpl in Heqf.
-        rewrite H in Heqf.
-        rewrite H0 in Heqf.
-        rewrite TPeqRefl in Heqf. easy. }
-      rewrite <- H1. apply TyUnbox.
-      apply TyFunApp. easy.
-      apply tagOfT in H0. rewrite H0.
-      destruct (TP2FCT T1) eqn:?; eauto using Typing.
-    + assert (TP2FCT T2 = Tstar).
-      { unfold tagOf in Heqf.
-        destruct (typeOf Γ (EPapp e1 e2)) eqn:?; try easy.
-        simpl in Heqo. rewrite H in Heqo. rewrite H0 in Heqo.
-        rewrite TPeqRefl in Heqo. congruence. }
-      rewrite H1. simpl. apply TyFunApp.
-      trivial. apply tagOfT in H0. rewrite H0.
-      destruct (TP2FCT T1) eqn:?; eauto using Typing.
+      eauto using IRTyping,InEq.
+  - destruct (tagOf Γ (PEApp e1 e2)) eqn:?;
+      rewrite (invertCall _ _ _ _ _ _ H H0 Heqi);
+      breakTagOf.
   - unfold Cast.
-    apply tagOfT in H. rewrite H.
-    destruct (TP2FCT T1) eqn:?;
-    destruct (TP2FCT T2) eqn:?; eauto using Typing.
-    destruct (dec_Tag t0 t); subst; try easy.
-    eauto using Typing.
+    breakTagOf;
+    destruct (TP2FCT T2) eqn:?...
+    destruct (dec_Tag t0 t); subst; try easy...
 Qed.
-
 
